WIP

src/Examples/AtomicPair/RefinementLog.v
@@ -26,6 +26,12 @@ Section refinement_triples.
 
   Import ExMach.
 
+  Record ghost_names :=
+    { γflag : gname;
+      γlog : gname;
+      γmain : gname;
+      γsrc : gname }.
+
   Definition someone_writing (p: nat * nat) (je: prodC natC (procTC (AtomicPair.Op))) :=
     (∃ (K: proc AtomicPair.Op unit → proc AtomicPair.Op (projT1 (snd je)))
         `{LanguageCtx AtomicPair.Op unit (projT1 (snd je)) AtomicPair.l K},
@@ -34,30 +40,31 @@ Section refinement_triples.
 
   (* If the commit flag is set, we can assume that *some* thread in the abstract
      program was in the middle of writing *)
-  Definition CommitInner γflag γlog :=
-    (∃ flag plog, own γflag (● (Excl' flag)) ∗ own γlog (● (Excl' plog))
+  Definition CommitInner (Γ: ghost_names) :=
+    (∃ flag plog, own (γflag Γ) (● (Excl' flag)) ∗ own (γlog Γ) (● (Excl' plog))
      ∗ log_commit d↦ fst flag ∗ log_fst d↦ (fst plog) ∗ log_snd d↦ (snd plog)
      ∗ (⌜ fst flag = 1 ⌝ → someone_writing plog (snd flag)))%I.
 
-  Definition MainInner γmain :=
-    (∃ (pcurr: nat * nat), own γmain (● (Excl' pcurr))
+  Definition MainInner (Γ: ghost_names) :=
+    (∃ (pcurr: nat * nat), own (γmain Γ) (● (Excl' pcurr))
                                ∗ main_fst d↦ (fst pcurr) ∗ main_snd d↦ (snd pcurr))%I.
 
-  Definition SrcInner γsrc :=
-    (∃ (psrc: nat * nat), own γsrc (● (Excl' psrc)) ∗ source_state psrc)%I.
+  Definition SrcInner (Γ: ghost_names) :=
+    (∃ (psrc: nat * nat), own (γsrc Γ) (● (Excl' psrc)) ∗ source_state psrc)%I.
 
-  Definition ExecInner γmain γflag γlog γsrc :=
-     (MainInner γmain ∗ CommitInner γflag γlog ∗ SrcInner γsrc)%I.
+  Definition ExecInner Γ :=
+     (MainInner Γ ∗ CommitInner Γ ∗ SrcInner Γ)%I.
 
   (* Holding the main lock guarantees the value of the atomic pair will not
      change out from underneath you -- this is enforced by granting ownership of
      appropriate ghost variables *)
-  Definition MainLockInv γmain γsrc :=
-    (∃ (pcurr: nat * nat), own γmain (◯ (Excl' pcurr)) ∗ own γsrc (◯ (Excl' pcurr)))%I.
+  Definition MainLockInv Γ :=
+    (∃ (pcurr: nat * nat), own (γmain Γ) (◯ (Excl' pcurr))
+                               ∗ own (γsrc Γ) (◯ (Excl' pcurr)))%I.
 
-  Definition LogLockInv γflag γlog :=
-    (∃ (plog: nat * nat), own γflag (◯ (Excl' (0, (0, existT _ (Ret tt) : procTC AtomicPair.Op))))
-                              ∗ own γlog (◯ (Excl' plog)))%I.
+  Definition LogLockInv Γ :=
+    (∃ (plog: nat * nat), own (γflag Γ) (◯ (Excl' (0, (0, existT _ (Ret tt) : procTC _))))
+                              ∗ own (γlog Γ) (◯ (Excl' plog)))%I.
 
   Definition mlN : namespace := (nroot.@"lock_main").
   Definition llN : namespace := (nroot.@"lock_log").
@@ -66,29 +73,39 @@ Section refinement_triples.
   Definition siN : namespace := (nroot.@"inner_src").
 
   Definition ExecInv :=
-    (source_ctx ρ
-     ∗ (∃ γlock_main γmain γsrc, is_lock mlN γlock_main main_lock (MainLockInv γmain γsrc)
-                                    ∗ inv miN (MainInner γmain)
-                                    ∗ inv siN (SrcInner γsrc))
-     ∗ (∃ γlock_log γflag γlog, is_lock llN γlock_log log_lock (LogLockInv γflag γlog)
-                                    ∗ inv liN (CommitInner γflag γlog)))%I.
+    (∃ Γ, source_ctx ρ
+      ∗ (∃ γlock_main, is_lock mlN γlock_main main_lock (MainLockInv Γ)
+                                    ∗ inv miN (MainInner Γ)
+                                    ∗ inv siN (SrcInner Γ))
+      ∗ (∃ γlock_log, is_lock llN γlock_log log_lock (LogLockInv Γ)
+                                    ∗ inv liN (CommitInner Γ)))%I.
 
-  Definition CrashStarter γmain γflag γsrc γlog :=
-    (main_lock m↦ 0 ∗ MainLockInv γmain γsrc
-               ∗ log_lock m↦ 0 ∗ LogLockInv γflag γlog)%I.
+  Definition CrashStarter Γ :=
+    (main_lock m↦ 0 ∗ log_lock m↦ 0 ∗
+      ∃ pcurr plog src,  
+        (∃ (pcurr: nat * nat), own (γmain Γ) (◯ (Excl' pcurr))
+                                   ∗ own (γsrc Γ) (◯ (Excl' pcurr)))%I.
 
-  Definition CrashInner γmain γflag γlog γsrc :=
-    (ExecInner γmain γflag γlog γsrc ∗ CrashStarter γmain γflag γlog γsrc)%I.
+  Definition LogLockInv Γ :=
+    (∃ (plog: nat * nat), own (γflag Γ) (◯ (Excl' (0, (0, existT _ (Ret tt) : procTC _))))
+                              ∗ own (γlog Γ) (◯ (Excl' plog)))%I.
 
-  Definition CrashInv γmain γflag γsrc γlog :=
-    (source_ctx ρ ∗ inv miN (MainInner γmain) ∗ inv siN (SrcInner γsrc)
-      ∗ inv liN (CommitInner γflag γlog))%I.
+
+               LogLockInv Γ)%I.
+
+  Definition CrashInner Γ :=
+    (ExecInner Γ ∗ CrashStarter Γ)%I.
+
+  Definition CrashInv Γ :=
+    (source_ctx ρ ∗ inv miN (MainInner Γ) ∗ inv siN (SrcInner Γ)
+      ∗ inv liN (CommitInner Γ))%I.
 
   Lemma write_refinement {T} j K `{LanguageCtx AtomicPair.Op unit T AtomicPair.l K} p:
     {{{ j ⤇ K (Call (AtomicPair.Write p)) ∗ ExecInv }}} write p {{{ v, RET v; j ⤇ K (Ret v) }}}.
   Proof.
-    iIntros (Φ) "(Hj&#Hsource_inv&#Hinv_main&#Hinv_log) HΦ".
-    iDestruct "Hinv_log" as (γlock_log γflag γlog) "(#Hlockinv&#Hinv)".
+    iIntros (Φ) "(Hj&Hrest) HΦ".
+    iDestruct "Hrest" as (Γ) "(#Hsource_inv&#Hinv_main&#Hinv_log)".
+    iDestruct "Hinv_log" as (γlock_log) "(#Hlockinv&#Hinv)".
     wp_bind. iApply (wp_lock with "[$]").
     iIntros "!> (Hlocked&HLL)".
     iDestruct "HLL" as (plog) "(Hflag_ghost&Hlog_ghost)".
@@ -97,7 +114,8 @@ Section refinement_triples.
     iInv "Hinv" as "H".
     destruct_commit_inner "H".
     iApply (wp_write_disk with "Hlog_fst"). iIntros "!> Hlog_fst".
-    iMod (ghost_var_update γlog (fst p, snd plog) with "Hlog_auth [$]") as "(Hlog_auth&Hlog_ghost)".
+    iMod (ghost_var_update (γlog Γ) (fst p, snd plog)
+            with "Hlog_auth [$]") as "(Hlog_auth&Hlog_ghost)".
     iModIntro.
     iExists (0, (0, existT _ (Ret tt) : procTC AtomicPair.Op)), _; iFrame.
     iSplitL ""; first by (simpl; iIntros "!> %"; congruence).
@@ -107,7 +125,7 @@ Section refinement_triples.
     iInv "Hinv" as "H".
     destruct_commit_inner "H".
     iApply (wp_write_disk with "Hlog_snd"). iIntros "!> Hlog_snd".
-    iMod (ghost_var_update γlog (fst p, snd p) with "Hlog_auth [$]") as "(Hlog_auth&Hlog_ghost)".
+    iMod (ghost_var_update (γlog Γ) (fst p, snd p) with "Hlog_auth [$]") as "(Hlog_auth&Hlog_ghost)".
     iModIntro.
     iExists (0, _), _; iFrame. iSplitL ""; first by (simpl; iIntros "!> %"; congruence).
     iClear "Hsomewriter".
@@ -116,7 +134,7 @@ Section refinement_triples.
     iInv "Hinv" as "H".
     destruct_commit_inner "H".
     iApply (wp_write_disk with "Hcommit"). iIntros "!> Hcommit".
-    iMod (ghost_var_update γflag
+    iMod (ghost_var_update (γflag Γ)
             (1, (j, (existT _ (K (Call (AtomicPair.Write p)))) : procTC AtomicPair.Op))
             with "Hflag_auth [$]") as "(Hflag_auth&Hflag_ghost)".
     iModIntro.
@@ -124,7 +142,7 @@ Section refinement_triples.
     { iNext. iIntros. simpl. iExists _, _. destruct p; eauto. }
     iClear "Hsomewriter".
 
-    iDestruct "Hinv_main" as (γlock_main γmain γsrc) "(#Hmlockinv&#Hminv&#Hmsrc)".
+    iDestruct "Hinv_main" as (γlock_main) "(#Hmlockinv&#Hminv&#Hmsrc)".
     wp_bind. iApply (wp_lock with "Hmlockinv").
     iIntros "!> (Hlocked'&HML)".
     iDestruct "HML" as (pmain) "(Hmain_ghost&Hsrc_ghost)".
@@ -133,7 +151,7 @@ Section refinement_triples.
     iInv "Hminv" as "H".
     destruct_main_inner "H".
     iApply (wp_write_disk with "Hmain_fst"). iIntros "!> Hmain_fst".
-    iMod (ghost_var_update γmain (fst p, snd pmain) with "Hmain_auth [$]")
+    iMod (ghost_var_update (γmain Γ) (fst p, snd pmain) with "Hmain_auth [$]")
       as "(Hmain_auth&Hmain_ghost)".
     iModIntro. iExists _. iFrame.
 
@@ -141,7 +159,7 @@ Section refinement_triples.
     iInv "Hminv" as "H".
     destruct_main_inner "H".
     iApply (wp_write_disk with "Hmain_snd"). iIntros "!> Hmain_snd".
-    iMod (ghost_var_update γmain (fst p, snd p) with "Hmain_auth [$]")
+    iMod (ghost_var_update (γmain Γ) (fst p, snd p) with "Hmain_auth [$]")
       as "(Hmain_auth&Hmain_ghost)".
     iModIntro. iExists _. iFrame.
 
@@ -155,8 +173,8 @@ Section refinement_triples.
     iMod (ghost_step_lifting with "Hj Hsource_inv Hsrc") as "(Hj&Hsrc&_)".
     { do 2 eexists; split; last by eauto. econstructor. }
     { solve_ndisj. }
-    iMod (ghost_var_update γsrc p with "Hsrc_auth [$]") as "(Hsrc_auth&Hsrc_ghost)".
-    iMod (ghost_var_update γflag (0, (0, existT _ (Ret tt) : procTC _))
+    iMod (ghost_var_update (γsrc Γ) p with "Hsrc_auth [$]") as "(Hsrc_auth&Hsrc_ghost)".
+    iMod (ghost_var_update (γflag Γ) (0, (0, existT _ (Ret tt) : procTC _))
             with "Hflag_auth [$]") as "(Hflag_auth&Hflag_ghost)".
     iModIntro.
     iExists _; iFrame.
@@ -180,8 +198,9 @@ Section refinement_triples.
   Lemma read_refinement {T} j K `{LanguageCtx AtomicPair.Op (nat*nat) T AtomicPair.l K}:
     {{{ j ⤇ K (Call (AtomicPair.Read)) ∗ ExecInv }}} read {{{ v, RET v; j ⤇ K (Ret v) }}}.
   Proof.
-    iIntros (Φ) "(Hj&#Hsource_inv&#Hinv_main&#Hinv_log) HΦ".
-    iDestruct "Hinv_main" as (γlock_main γmain γsrc) "(#Hmlockinv&#Hminv&#Hmsrc)".
+    iIntros (Φ) "(Hj&Hrest) HΦ".
+    iDestruct "Hrest" as (Γ) "(#Hsource_inv&#Hinv_main&#Hinv_log)".
+    iDestruct "Hinv_main" as (γlock_main) "(#Hmlockinv&#Hminv&#Hmsrc)".
     wp_bind. iApply (wp_lock with "Hmlockinv").
     iIntros "!> (Hlocked'&HML)".
     iDestruct "HML" as (pmain) "(Hmain_ghost&Hsrc_ghost)".
@@ -265,6 +284,140 @@ Section refinement.
                                         (rec_singleton recv) σ1c (Val σ2c res) →
     ∃ σ2a, AtomicPair.l.(proc_exec_seq) es (rec_singleton (Ret tt)) σ1a (Val σ2a res).
   Proof.
-  Abort.
+    eapply (exmach_crash_refinement_seq) with
+        (Σ := myΣ)
+        (exec_inv := fun H1 H2 => (∃ ρ, @ExecInv myΣ H2 _ H1 _ _ ρ)%I)
+        (exec_inner := fun H1 H2 =>
+                         (∃ Γ v1 v2, main_lock m↦ v1 ∗log_lock m↦ v2 ∗
+                                         (⌜ v1 = 0  ⌝ -∗ @MainLockInv myΣ _ Γ) ∗
+                                         (⌜ v2 = 0  ⌝ -∗ @LogLockInv myΣ _ _ Γ) ∗
+                                         @ExecInner myΣ H2 H1 _ _ Γ)%I)
+        (crash_inner := fun H1 H2 => (∃ Γ, @CrashInner myΣ H2 H1 _ _ Γ)%I)
+        (crash_param := fun H1 H2 => ghost_names)
+        (crash_inv := fun H1 H2 Γ =>(∃ ρ, @CrashInv myΣ H2 H1 _ _ ρ Γ)%I)
+        (crash_starter := fun H1 H2 Γ => (@CrashStarter myΣ _ _ _ Γ)%I)
+        (E := nclose sourceN).
+    { apply _. }
+    { apply _. }
+    { intros. apply _. }
+    { intros. apply _. }
+    { set_solver+. }
+    { intros. iIntros "(?&H)". iDestruct "H" as (ρ) "H". destruct op.
+      - iApply (write_refinement with "[$]"). eauto.
+      - iApply (read_refinement with "[$]"). eauto.
+    }
+    { intros. iIntros "H". iDestruct "H" as (ρ ?) "(?&?)". eauto. }
+    {
+      (* recv triple TODO: pull this triple out? *)
+      intros ? ? Γ. iIntros "(H&Hstarter)". iDestruct "H" as (ρ) "(#Hctx&#Hrest)".
+      iDestruct "Hrest" as "(#Hinv_main&#Hsource_inv&#Hinv_log)".
+      iDestruct "Hstarter" as "(Hmain_lock&Hmain_lock_inv&Hlog_lock&Hlog_lock_inv)".
+      iDestruct "Hlog_lock_inv" as (plog) "(Hflag_ghost&Hlog_ghost)".
+      iDestruct "Hmain_lock_inv" as (pmain) "(Hmain_ghost&Hsrc_ghost)".
+      wp_bind.
+      iInv "Hinv_log" as "H".
+      destruct_commit_inner "H".
+
+      iApply (wp_read_disk with "Hcommit"); iIntros "!> Hcommit".
+      simpl.
+      iModIntro.
+
+      iDestruct "Hinv
+
+
+
+
+      wp_ret. iInv "Hinv" as (ptr_val pcurr pother) ">(?&Hcase&?)" "_".
+      iMod (own_alloc (● (Excl' ptr_val) ⋅ ◯ (Excl' ptr_val))) as (γ1) "[Hauth_ptr Hfrag_ptr]".
+      { apply auth_valid_discrete_2; split; eauto. econstructor. }
+      iMod (own_alloc (● (Excl' pcurr) ⋅ ◯ (Excl' pcurr))) as (γ2) "[Hauth_curr Hfrag_curr]".
+      { by eauto. }
+      iMod (own_alloc (● (Excl' pother) ⋅ ◯ (Excl' pother))) as (γ3) "[Hauth_other Hfrag_other]".
+      { by eauto. }
+      iApply (fupd_mask_weaken _ _).
+      { solve_ndisj. }
+      iExists pcurr, pcurr. iFrame.
+      iSplitL "".
+      { iPureIntro; econstructor. }
+      iClear "Hctx Hinv".
+      iIntros (???) "(#Hctx&Hstate)".
+      iModIntro. iExists _. iFrame. iExists γ1, γ2, γ3.
+      iSplitL "Hfrag_ptr Hfrag_curr Hfrag_other"; iIntros; iExists _, _, _; iFrame.
+    }
+    { intros ?? (H&?). inversion H. subst. eapply ExMach.init_state_wf. }
+    { intros ??? (H&Hinit) ??. inversion H. inversion Hinit. subst.
+      iIntros "(Hmem&Hdisk&#?&Hstate)".
+      iMod (own_alloc (● (Excl' 0) ⋅ ◯ (Excl' 0))) as (γ1) "[Hauth_ptr Hfrag_ptr]".
+      { apply auth_valid_discrete_2; split; eauto. econstructor. }
+      iMod (own_alloc (● (Excl' (0, 0)) ⋅ ◯ (Excl' (0, 0)))) as (γ2) "[Hauth_curr Hfrag_curr]".
+      { apply auth_valid_discrete_2; split; eauto. econstructor. }
+      iMod (own_alloc (● (Excl' (0, 0)) ⋅ ◯ (Excl' (0, 0)))) as (γ3) "[Hauth_other Hfrag_other]".
+      { apply auth_valid_discrete_2; split; eauto. econstructor. }
+      iPoseProof (init_mem_split with "Hmem") as "?".
+      iPoseProof (init_disk_split with "Hdisk") as "(?&?&?&?&?)".
+      iModIntro. iExists _. iFrame. iExists γ1, γ2, γ3.
+      iSplitL "Hfrag_ptr Hfrag_curr Hfrag_other"; iIntros; iExists _, _, _; iFrame.
+      simpl. iFrame.
+    }
+    { intros. iIntros "H". iDestruct "H" as (ρ) "(#Hctx&#Hinv)".
+      iDestruct "Hinv" as (γlock γ1 γ2 γ3) "(#Hlock&#Hinv)".
+      iInv "Hinv" as "Hopen" "_".
+      destruct_einner "Hopen".
+      iApply fupd_mask_weaken; first by solve_ndisj.
+      iIntros (?) "Hmem".
+      iModIntro. iExists _, _, _. iFrame.
+      iPoseProof (@init_mem_split with "Hmem") as "?".
+      iFrame.
+    }
+    { intros. iIntros "H". iDestruct "H" as (ρ) "(#Hctx&#Hinv)".
+      iInv "Hinv" as ">Hopen" "_".
+      iDestruct "Hopen" as (???) "(?&?&_)".
+      iApply fupd_mask_weaken; first by solve_ndisj.
+      iIntros (?) "Hmem".
+      iModIntro. iExists _, _, _. iFrame.
+      iPoseProof (@init_mem_split with "Hmem") as "?".
+      iFrame.
+    }
+    { intros. iIntros "H". iDestruct "H" as "(Hinv&#Hsrc)".
+      iDestruct "Hinv" as (invG) "Hinv".
+      iDestruct "Hinv" as (???) "(?&?&?)".
+      iMod (@inv_alloc myΣ (exm_invG) iN _ CrashInner with "[-]").
+      { iNext. iExists _, _, _; iFrame. }
+      iModIntro. iFrame. iExists tt, _. iFrame "Hsrc".
+    }
+    { intros. iIntros "H". iDestruct "H" as "(Hinv&#Hsrc)".
+      iDestruct "Hinv" as (invG v) "Hinv".
+      iDestruct "Hinv" as "(?&Hinv)".
+      iDestruct "Hinv" as (γ1 γ2 γ3) "(Hlock&Hinner)".
+      iMod (@lock_init myΣ (ExMachG _ (exm_invG) (exm_mem_inG) (exm_disk_inG)) _ lN
+                       lock_addr _ (ExecLockInv γ1 γ2 γ3) with "[$] [-Hinner]") as (γlock) "H".
+      { iFrame. }
+      iMod (@inv_alloc myΣ (exm_invG) iN _ (ExecInner γ1 γ2 γ3) with "[Hinner]").
+      { iFrame. }
+      iModIntro. iExists cfg. iFrame "Hsrc". iExists _, _, _, _. iFrame.
+    }
+    { iIntros (??) "H".
+      iDestruct "H" as (?) "(?&H)".
+      iDestruct "H" as (????) "(?&Hinv)".
+      iInv "Hinv" as "H" "_".
+      destruct_einner "H".
+      iApply fupd_mask_weaken; first by solve_ndisj.
+      iExists _; iFrame.
+    }
+    { iIntros (??) "H".
+      iDestruct "H" as (?) "(?&H)".
+      iDestruct "H" as (????) "(Hlock&Hinv)".
+      iInv "Hinv" as "H" "_".
+      destruct_einner "H".
+      iMod (lock_crack with "Hlock") as ">H"; first by solve_ndisj.
+      iDestruct "H" as (v) "(?&?)".
+      iApply fupd_mask_weaken; first by solve_ndisj.
+      iExists _; iFrame.
+      iFrame. iIntros (???) "(?&?)".
+      iModIntro.
+      iExists _. iFrame. iExists _, _, _. iFrame.
+      iExists _, _, _. iFrame.
+    }
+  Qed.
 
 End refinement.
